Refactor sim_module, two admits on init_locals

coq/proof/SimulationModule.v
@@ -217,131 +217,416 @@ Proof.
   apply HYPB; ss.
 Qed.
 
+Lemma transl_products_init
+      l ndts prods_src prods_tgt
+      (TRANSL_PRODUCTS:
+         transl_products (module_intro l ndts prods_src)
+                         (module_intro l ndts prods_tgt) prods_src prods_tgt)
+      conf_src st_src
+      main args
+      (INIT: s_genInitState [module_intro l ndts prods_src] main args Mem.empty =
+             Some (conf_src, st_src))
+  :
+    exists conf_tgt st_tgt,
+    <<INIT: s_genInitState [module_intro l ndts prods_tgt] main args Mem.empty =
+             Some (conf_tgt, st_tgt)>>
+.
+Proof.
+  unfold s_genInitState in INIT. des_ifs.
+  ss. des_ifs.
+  expl transl_products_lookupFdefViaIDFromProducts. ss. rename products5 into prods_src.
+  unfold s_genInitState. ss.
+  rewrite TGT.
+  match goal with
+  | [|- context [productInModuleB_dec ?a ?b]] => destruct (productInModuleB_dec a b)
+  end; simtac; cycle 1.
+  { apply infrastructure_props.lookupFdefViaIDFromProducts_inv in TGT. congruence. }
+  unfold initTargetData in *. ss.
+  rename Heq1 into INITMEM.
+  erewrite <- transl_products_genGlobalAndInitMem; eauto. rewrite INITMEM.
+  abstr (module_intro layouts5 namedts5 prods_src) md_src.
+  abstr (module_intro layouts5 namedts5 prods_tgt) md_tgt.
+  rename Heq3 into INIT_LOCALS.
+  clear - FDEF INIT_LOCALS.
+  inv FDEF.
+  - inv NOP_FDEF. ss. inv BLOCKS. des_ifs_safe ss. des. clarify.
+    esplits; eauto.
+  - inv VALID_FDEF. des_ifs_safe ss.
+    des_bool. des_sumbool. clarify.
+    rewrite INIT_LOCALS.
+    esplits; eauto.
+Qed.
+
+Definition init_invmem (m0: mem): InvMem.Rel.t :=
+  InvMem.Rel.mk (InvMem.Unary.mk [] Mem.empty [] m0.(Mem.nextblock))
+                (InvMem.Unary.mk [] Mem.empty [] m0.(Mem.nextblock))
+                (Mem.nextblock m0 - 1)
+                (memory_props.MemProps.inject_init (Mem.nextblock m0 - 1))
+.
+
+Lemma init_mem_sem
+      (* Do we need prods_src/prods_tgt both? not sure, but this form is sufficient *)
+      (* l ndts prods gl fs m0 *)
+      (* (INIT: genGlobalAndInitMem (l, ndts) prods [] [] Mem.empty = ret (gl, fs, m0)) *)
+      l ndts prods_src prods_tgt gl fs m0
+      (INIT_SRC: genGlobalAndInitMem (l, ndts) prods_src [] [] Mem.empty = ret (gl, fs, m0))
+      (INIT_TGT: genGlobalAndInitMem (l, ndts) prods_tgt [] [] Mem.empty = ret (gl, fs, m0))
+      lc args params
+      (INIT_LOCALS: initLocals (l, ndts) args params = ret lc)
+      sys_src sys_tgt
+  :
+      <<SEM: InvMem.Rel.sem
+               (mkCfg sys_src (l, ndts) prods_src gl fs)
+               (mkCfg sys_tgt (l, ndts) prods_tgt gl fs)
+               m0 m0 (init_invmem m0)>>
+.
+Proof.
+  hexploit genGlobalAndInitMem__wf_globals_Mem; eauto; intro WF; des.
+  unfold initTargetData in *.
+  econs; ss; eauto.
+  - econs; ss; eauto.
+    + eapply memory_props.MemProps.redundant__wf_globals; eauto.
+    + ii. ss.
+    + econs; eauto.
+    + eapply Pos.le_1_l; eauto.
+  - econs; ss; eauto.
+    + eapply memory_props.MemProps.redundant__wf_globals; eauto.
+    + ii. ss.
+    + econs; eauto.
+    + eapply Pos.le_1_l; eauto.
+Qed.
+
 Lemma transl_sim_module:
   transl_module <2= sim_module.
 Proof.
   s. intros module_src module_tgt MODULE.
   inv MODULE.
   ii.
-  expl s_genInitState__opsem_wf (try exact WF_SRC; eauto).
-  apply_all_once wf_ConfigI_spec. apply_all_once wf_StateI_spec.
-  (* Without this, prop will be destructed into multiple parts, and readibility is marred. *)
-  unfold s_genInitState in SRC. simtac.
-  clear COND e0. apply infrastructure_props.InProductsB_In in e.
-  exploit transl_products_lookupFdefViaIDFromProducts; eauto. i. des.
-  destruct fdef_tgt. unfold LLVMinfra.is_true in *. simtac.
-  destruct fheader5.
-  (* TODO: define all_with_term_once *)
-  (* Ltac expl_with H := expl lookupFdefViaIDFromProducts_ideq (idtac H; try exact H; eauto). *)
-  (* all_with_term expl_with lookupFdefViaIDFromProducts. *)
-  expl lookupFdefViaIDFromProducts_ideq (try exact COND3; eauto). clarify.
-  expl lookupFdefViaIDFromProducts_ideq (try exact TGT; eauto). clarify.
-  inv FDEF.
-  { inv NOP_FDEF.
-    assert (NOP_BLOCKS_ENTRY:
-              exists phi' cmds' term' b',
-                blocks5 = ((l0, stmts_intro phi' cmds' term')::b')).
-    { inv BLOCKS.
-      destruct y. destruct s.
-      assert (LEQ: l1 = l0).
-      {
-        exploit transl_products_lookupFdefViaIDFromProducts; eauto. i. des.
-        clarify.
+  {
+    pose (s_genInitState [module_intro l_src ndts_src prods_src] main args0 Mem.empty)
+      as SRC_INIT.
+    pose st_src as SRC_ST.
+
+    remember (s_genInitState [module_intro l_tgt ndts_tgt prods_tgt]
+                             main args0 Mem.empty) as TI eqn:TGT_INIT0.
+    pose (s_genInitState [module_intro l_tgt ndts_tgt prods_tgt]
+                         main args0 Mem.empty) as TGT_INIT1.
+    assert(EQ: TI = TGT_INIT1) by  ss. rewrite EQ. clarify.
+    unfold s_genInitState in SRC, EQ.
+    ss.
+    des_ifs_safe ss. clarify. rename products5 into prods_src.
+    expl transl_products_lookupFdefViaIDFromProducts.
+    rewrite TGT in *. ss.
+    match goal with
+    | [H: context [productInModuleB_dec ?a ?b] |- _] => destruct (productInModuleB_dec a b)
+    end; cycle 1.
+    { apply infrastructure_props.lookupFdefViaIDFromProducts_inv in TGT. ss. congruence. }
+    unfold initTargetData in *. ss.
+    rename Heq2 into INITMEM.
+    unfold proj_sumbool in *. des_ifs_safe ss. clarify.
+    erewrite <- transl_products_genGlobalAndInitMem in EQ; eauto. rewrite INITMEM in *.
+    rename Heq10 into INIT_LOCALS.
+    (* clear - FDEF INIT_LOCALS. *)
+    inv FDEF.
+
+
+
+    - (* fheader_intro is different here *)
+      (* actually, it is same and this fact is needed for nop_sim_fdef. *)
+      (* this fact can only be achieved by *)
+      (* inv NOP_FDEF. so I save nop_fdef here, and then inv *)
+      (* TODO: generalize nop_sim_fdef, header -> header_src/header_tgt. anyhow they are same *)
+      (* by nop_fdef in premise *)
+      inversion NOP_FDEF; subst.
+      ss. inv BLOCKS. des_ifs_safe ss. des. clarify.
+      hexploit nop_sim_fdef; try exact NOP_FDEF.
+      { instantiate (1:= {|
+                          CurSystem := [module_intro l_tgt ndts_tgt prods_tgt];
+                          CurTargetData := (l_tgt, ndts_tgt);
+                          CurProducts := prods_tgt;
+                          Globals := g;
+                          FunTable := g0 |}).
+        instantiate (1:= {|
+                          CurSystem := [module_intro l_tgt ndts_tgt prods_src];
+                          CurTargetData := (l_tgt, ndts_tgt);
+                          CurProducts := prods_src;
+                          Globals := g;
+                          FunTable := g0 |}).
+        ss.
       }
-      subst.
+      { ss. }
+      intro SIM; des.
+
+
+
+
+
+
+
+      hexploit genGlobalAndInitMem__wf_globals_Mem; eauto; []; intro WF; des.
+      unfold sim_fdef in *.
+      hexploit SIM.
+      { eapply init_mem_sem; eauto.
+        erewrite <- transl_products_genGlobalAndInitMem; eauto.
+      }
+      { instantiate (1:= args0).
+        instantiate (1:= args0).
+        ss.
+        rename Heq1 into INIT_LOCALS.
+        (* OpsemPP.wf_ExecutionContext__at_beginning_of_function *)
+        clear - WF4 WF INIT_LOCALS.
+        (* OpsemPP.initLocals_spec' *)
+        (* opsem_props.OpsemProps.initLocals_spec *)
+        admit.
+      }
+      {
+        (* instantiate *)
+        (*   (1:= *)
+        (*      {| *)
+        (*        CurFunction := fdef_intro *)
+        (*                         (fheader_intro fnattrs0 typ0 id0 args1 varg0) *)
+        (*                         ((l1, stmts_intro phinodes0 cmds5 terminator0) :: b1); *)
+        (*        CurBB := (l1, stmts_intro phinodes0 cmds5 terminator0); *)
+        (*        CurCmds := cmds5; *)
+        (*        Terminator := terminator0; *)
+        (*        Locals := g1; *)
+        (*        Allocas := [] |}). *)
+        econs; ss; eauto.
+      }
+      clear SIM. intro SIM_LOCAL; des.
+      inv SIM_LOCAL. ss. clarify.
+
+
+
+
       esplits; eauto.
-    }
-    des.
-
-
-
-    expl genGlobalAndInitMem__wf_globals_Mem.
-
-    do 3 eexists.
-    apply dependent_split.
-    - unfold s_genInitState. ss. rewrite TGT.
-      match goal with
-      | [|- context [productInModuleB_dec ?a ?b]] => destruct (productInModuleB_dec a b)
-      end; simtac; cycle 1.
-      { apply infrastructure_props.lookupFdefViaIDFromProducts_inv in TGT. congruence. }
-      unfold initTargetData in *.
-      erewrite <- transl_products_genGlobalAndInitMem; eauto. rewrite COND1.
-      rewrite COND2.
-      eauto.
-    - i; des.
-
-      clear s_genInitState__opsem_wf.
-      hexploit s_genInitState__opsem_wf; eauto; []; intro WF_TGT2; destruct WF_TGT2 as [WF_CONF_TGT WF_ST_TGT].
-      apply wf_ConfigI_spec in WF_CONF_TGT. apply wf_StateI_spec in WF_ST_TGT.
-
-      apply sim_local_lift_sim.
-      { eapply transl_products_sim_conf; eauto. }
-      econs; ss.
-      + econs.
-      + apply nop_sim.
+      + eapply sim_local_lift_sim; eauto.
+        { eapply transl_products_sim_conf; eauto.
+          subst TGT_INIT1.
+          expl s_genInitState__opsem_wf.
+          eapply wf_ConfigI_spec; eauto.
+        }
+        econs; ss; eauto.
         * econs; eauto.
-        * clarify.
-          inv BLOCKS. des. clarify.
-          econs; eauto.
-          { econs; eauto.
-            econs; eauto. }
-          { econs. esplits; eauto.
-            exact (SF_ADMIT "inject_locals"). }
-          { econs. }
-          { exact (SF_ADMIT "init mem"). }
-          { ss. }
-          { ss. }
-      + reflexivity.
-  }
-  { ss. simtac.
-    inv e0.
-    expl genGlobalAndInitMem__wf_globals_Mem.
-    do 3 eexists. apply dependent_split.
-    - unfold s_genInitState. ss. rewrite TGT.
-      match goal with
-      | [|- context [productInModuleB_dec ?a ?b]] => destruct (productInModuleB_dec a b)
-      end; simtac; cycle 1.
-      { apply infrastructure_props.lookupFdefViaIDFromProducts_inv in TGT. congruence. }
-      unfold initTargetData in *.
-      erewrite <- transl_products_genGlobalAndInitMem; eauto. rewrite COND1.
-      rewrite COND2. eauto.
-    - i; des.
+        * eapply SIM_LOCAL0.
+          { (* wf *)
+            subst TGT_INIT1.
+            expl s_genInitState__opsem_wf.
+            split; ss.
+          }
+        * reflexivity.
 
-      clear s_genInitState__opsem_wf.
-      hexploit s_genInitState__opsem_wf; eauto; []; intro WF_TGT2; destruct WF_TGT2 as [WF_CONF_TGT WF_ST_TGT].
-      apply wf_ConfigI_spec in WF_CONF_TGT. apply wf_StateI_spec in WF_ST_TGT.
 
-      apply sim_local_lift_sim.
-      { eapply transl_products_sim_conf; eauto. }
-      econs; ss.
-      + econs.
-      + generalize VALID_FDEF. i.
-        unfold forallb2AL in VALID_FDEF0. ss. apply andb_true_iff in VALID_FDEF0.
-        repeat (des; des_bool; des_sumbool; des_ifs_safe).
-        hexploit InvState.Rel.sem_empty; eauto.
-        { exact (SF_ADMIT "init_locals inject_locals"). }
-        i. des.
-        apply valid_sim. econs; eauto.
-        * ss.
-        *
-          cbn in *.
-          clear_tac.
-          unfold Debug.failwith_false in *.
-          repeat multimatch goal with
-                 | H:context [id_dec ?a ?b] |- _ => destruct (id_dec a b); ss
-                 end.
-          repeat (des; des_bool; des_sumbool; des_ifs_safe).
-        (* inject allocas *)
-        (* * ss. econs; eauto. *)
-        * ss. des_ifsH Heq0.
-          { exists []. ss. }
-          { eexists; eauto. }
-        * ss. exact (SF_ADMIT "InvMem.Rel.sem init_mem").
-      + reflexivity.
-  }
-Unshelve.
-{ apply empty_invmem. }
-{ by econs; eauto. }
-{ apply empty_invmem. }
+
+    - destruct blocks5.
+      { ss. des_ifs. }
+      assert(args5 = args1).
+      { ss. des_ifs_safe ss. des_bool. unfold proj_sumbool in *. des_ifs. }
+      clarify.
+      rewrite INIT_LOCALS in *.
+      des_ifs.
+      (* I want "TGT_INIT1 = Some" without breaking VALID_FDEF *)
+      (* both "TGT_INIT1 = Soem" && VALID_FDEF is used in next hexploit *)
+      (* TODO: can we do this in more smart way? *)
+      (* Here, even "ss" breaks VALID_FDEF. It is really truly annoying *)
+      hexploit valid_sim_fdef; try exact VALID_FDEF.
+      { instantiate (1:= {|
+                          CurSystem := [module_intro l_tgt ndts_tgt prods_tgt];
+                          CurTargetData := (l_tgt, ndts_tgt);
+                          CurProducts := prods_tgt;
+                          Globals := g;
+                          FunTable := g0 |}).
+        instantiate (1:= {|
+                          CurSystem := [module_intro l_tgt ndts_tgt prods_src];
+                          CurTargetData := (l_tgt, ndts_tgt);
+                          CurProducts := prods_src;
+                          Globals := g;
+                          FunTable := g0 |}).
+        ss.
+      }
+      { subst TGT_INIT1.
+        expl s_genInitState__opsem_wf.
+        ss.
+      }
+      intro SIM; des.
+
+
+
+      ss. des_ifs_safe ss. clarify. des. des_bool. unfold is_empty in *. des_ifs_safe ss.
+      unfold proj_sumbool in *. des_ifs_safe ss. des_ifs_safe. clear_tac.
+
+
+
+
+
+
+
+
+      hexploit genGlobalAndInitMem__wf_globals_Mem; eauto; []; intro WF; des.
+      unfold sim_fdef in *.
+      hexploit SIM.
+      { eapply init_mem_sem; eauto.
+        erewrite <- transl_products_genGlobalAndInitMem; eauto.
+      }
+      { instantiate (1:= args0).
+        instantiate (1:= args0).
+        ss.
+        (* OpsemPP.wf_ExecutionContext__at_beginning_of_function *)
+        clear - WF4 WF INIT_LOCALS.
+        (* OpsemPP.initLocals_spec' *)
+        (* opsem_props.OpsemProps.initLocals_spec *)
+        admit.
+      }
+      { econs; ss; eauto. }
+      clear SIM. intro SIM_LOCAL; des.
+      inv SIM_LOCAL. ss. clarify.
+
+
+
+
+      esplits; eauto.
+      + eapply sim_local_lift_sim; eauto.
+        { eapply transl_products_sim_conf; eauto.
+          subst TGT_INIT1.
+          expl s_genInitState__opsem_wf.
+          eapply wf_ConfigI_spec; eauto.
+        }
+        econs; ss; eauto.
+        * econs; eauto.
+        * eapply SIM_LOCAL0.
+          { (* wf *)
+            subst TGT_INIT1.
+            expl s_genInitState__opsem_wf.
+            split; ss.
+          }
+        * reflexivity.
+Admitted.
+
+(* Lemma transl_sim_module: *)
+(*   transl_module <2= sim_module. *)
+(* Proof. *)
+(*   s. intros module_src module_tgt MODULE. *)
+(*   inv MODULE. *)
+(*   ii. *)
+(*   expl s_genInitState__opsem_wf (try exact WF_SRC; eauto). *)
+(*   apply_all_once wf_ConfigI_spec. apply_all_once wf_StateI_spec. *)
+(*   (* Without this, prop will be destructed into multiple parts, and readibility is marred. *) *)
+(*   unfold s_genInitState in SRC. simtac. *)
+(*   clear COND e0. apply infrastructure_props.InProductsB_In in e. *)
+(*   exploit transl_products_lookupFdefViaIDFromProducts; eauto. i. des. *)
+(*   destruct fdef_tgt. unfold LLVMinfra.is_true in *. simtac. *)
+(*   destruct fheader5. *)
+(*   (* TODO: define all_with_term_once *) *)
+(*   (* Ltac expl_with H := expl lookupFdefViaIDFromProducts_ideq (idtac H; try exact H; eauto). *) *)
+(*   (* all_with_term expl_with lookupFdefViaIDFromProducts. *) *)
+(*   expl lookupFdefViaIDFromProducts_ideq (try exact COND3; eauto). clarify. *)
+(*   expl lookupFdefViaIDFromProducts_ideq (try exact TGT; eauto). clarify. *)
+(*   inv FDEF. *)
+(*   { inv NOP_FDEF. *)
+(*     assert (NOP_BLOCKS_ENTRY: *)
+(*               exists phi' cmds' term' b', *)
+(*                 blocks5 = ((l0, stmts_intro phi' cmds' term')::b')). *)
+(*     { inv BLOCKS. *)
+(*       destruct y. destruct s. *)
+(*       assert (LEQ: l1 = l0). *)
+(*       { *)
+(*         exploit transl_products_lookupFdefViaIDFromProducts; eauto. i. des. *)
+(*         clarify. *)
+(*       } *)
+(*       subst. *)
+(*       esplits; eauto. *)
+(*     } *)
+(*     des. *)
+
+
+
+(*     expl genGlobalAndInitMem__wf_globals_Mem. *)
+
+(*     do 3 eexists. *)
+(*     apply dependent_split. *)
+(*     - unfold s_genInitState. ss. rewrite TGT. *)
+(*       match goal with *)
+(*       | [|- context [productInModuleB_dec ?a ?b]] => destruct (productInModuleB_dec a b) *)
+(*       end; simtac; cycle 1. *)
+(*       { apply infrastructure_props.lookupFdefViaIDFromProducts_inv in TGT. congruence. } *)
+(*       unfold initTargetData in *. *)
+(*       erewrite <- transl_products_genGlobalAndInitMem; eauto. rewrite COND1. *)
+(*       rewrite COND2. *)
+(*       eauto. *)
+(*     - i; des. *)
+
+(*       clear s_genInitState__opsem_wf. *)
+(*       hexploit s_genInitState__opsem_wf; eauto; []; intro WF_TGT2; destruct WF_TGT2 as [WF_CONF_TGT WF_ST_TGT]. *)
+(*       apply wf_ConfigI_spec in WF_CONF_TGT. apply wf_StateI_spec in WF_ST_TGT. *)
+
+(*       apply sim_local_lift_sim. *)
+(*       { eapply transl_products_sim_conf; eauto. } *)
+(*       econs; ss. *)
+(*       + econs. *)
+(*       + apply nop_sim. *)
+(*         * econs; eauto. *)
+(*         * clarify. *)
+(*           inv BLOCKS. des. clarify. *)
+(*           econs; eauto. *)
+(*           { econs; eauto. *)
+(*             econs; eauto. } *)
+(*           { econs. esplits; eauto. *)
+(*             exact (SF_ADMIT "inject_locals"). } *)
+(*           { econs. } *)
+(*           { exact (SF_ADMIT "init mem"). } *)
+(*           { ss. } *)
+(*           { ss. } *)
+(*       + reflexivity. *)
+(*   } *)
+(*   { ss. simtac. *)
+(*     inv e0. *)
+(*     expl genGlobalAndInitMem__wf_globals_Mem. *)
+(*     do 3 eexists. apply dependent_split. *)
+(*     - unfold s_genInitState. ss. rewrite TGT. *)
+(*       match goal with *)
+(*       | [|- context [productInModuleB_dec ?a ?b]] => destruct (productInModuleB_dec a b) *)
+(*       end; simtac; cycle 1. *)
+(*       { apply infrastructure_props.lookupFdefViaIDFromProducts_inv in TGT. congruence. } *)
+(*       unfold initTargetData in *. *)
+(*       erewrite <- transl_products_genGlobalAndInitMem; eauto. rewrite COND1. *)
+(*       rewrite COND2. eauto. *)
+(*     - i; des. *)
+
+(*       clear s_genInitState__opsem_wf. *)
+(*       hexploit s_genInitState__opsem_wf; eauto; []; intro WF_TGT2; destruct WF_TGT2 as [WF_CONF_TGT WF_ST_TGT]. *)
+(*       apply wf_ConfigI_spec in WF_CONF_TGT. apply wf_StateI_spec in WF_ST_TGT. *)
+
+(*       apply sim_local_lift_sim. *)
+(*       { eapply transl_products_sim_conf; eauto. } *)
+(*       econs; ss. *)
+(*       + econs. *)
+(*       + generalize VALID_FDEF. i. *)
+(*         unfold forallb2AL in VALID_FDEF0. ss. apply andb_true_iff in VALID_FDEF0. *)
+(*         repeat (des; des_bool; des_sumbool; des_ifs_safe). *)
+(*         hexploit InvState.Rel.sem_empty; eauto. *)
+(*         { exact (SF_ADMIT "init_locals inject_locals"). } *)
+(*         i. des. *)
+(*         apply valid_sim. econs; eauto. *)
+(*         * ss. *)
+(*         * *)
+(*           cbn in *. *)
+(*           clear_tac. *)
+(*           unfold Debug.failwith_false in *. *)
+(*           repeat multimatch goal with *)
+(*                  | H:context [id_dec ?a ?b] |- _ => destruct (id_dec a b); ss *)
+(*                  end. *)
+(*           repeat (des; des_bool; des_sumbool; des_ifs_safe). *)
+(*         (* inject allocas *) *)
+(*         (* * ss. econs; eauto. *) *)
+(*         * ss. des_ifsH Heq0. *)
+(*           { exists []. ss. } *)
+(*           { eexists; eauto. } *)
+(*         * ss. exact (SF_ADMIT "InvMem.Rel.sem init_mem"). *)
+(*       + reflexivity. *)
+(*   } *)
+(* Unshelve. *)
+(* { apply empty_invmem. } *)
+(* { by econs; eauto. } *)
+(* { apply empty_invmem. } *)
+(* (* Qed. *) *)
 (* Qed. *)
-Qed.
